wow such proofs

Projects.v
@@ -1,41 +1,57 @@
+Require Import Omega.
 
-Inductive Project : Type :=
+Inductive Project : Set :=
 | Task : nat -> Project
 | Sum : Project -> Project -> Project
 | Prod : Project -> Project -> Project
+| Seq : Project -> Project -> Project
 .
 
-Inductive Exec : Project -> Prop :=
-| ETask : forall n, Exec (Task n)
-| ESumLeft : forall a b, Exec a -> Exec (Sum a b)
-| ESumRight : forall a b, Exec b -> Exec (Sum a b)
-| EProd : forall a b, Exec a -> Exec b -> Exec (Prod a b)
+Inductive Exec : Project -> nat -> nat -> Type :=
+| ETask : forall (tid ord : nat), Exec (Task tid) ord ord
+| ESumLeft : forall a b lo hi, Exec a lo hi -> Exec (Sum a b) lo hi
+| ESumRight : forall a b lo hi, Exec b lo hi -> Exec (Sum a b) lo hi
+| EProd : forall a b loA loB hiA hiB,
+    Exec a loA hiA ->
+    Exec b loB hiB ->
+    Exec (Prod a b) (min loA loB) (max hiA hiB)
+| ESeq : forall a b loA loB hiA hiB,
+    Exec a loA hiA ->
+    Exec b loB hiB ->
+    hiA < loB      ->
+    Exec (Seq a b) loA hiB
 .
-
-(* Fixpoint execLeft (p : Project) : Exec p := *)
-(*   match p with *)
-(*   | Task n => ETask n *)
-(*   | Sum a b => ESumLeft a b (execLeft a) *)
-(*   | Prod a b => EProd a b (execLeft a) (execLeft b) *)
-(*   end *)
-(*   . *)
 
 (* a is less than b. If b is executed, then a is also executed *)
-Definition projLe a b : Prop := Exec b -> Exec a.
+Definition projLe a b : Type := forall lo hi, Exec b lo hi -> Exec a lo hi.
 
-Bind Scope project with Project.
-Delimit Scope project with proj.
-Open Scope project.
+Definition projGe a b : Type := forall lo hi, Exec a lo hi -> Exec b lo hi.
 
-Notation "a ':+' b" := (Sum a b) (right associativity, at level 55) : project.
+Definition projE a b : Type := projLe a b * projGe a b.
 
-Notation "a ':*' b" := (Prod a b) (right associativity, at level 45) : project.
+Bind Scope proj_scope with Project.
+Delimit Scope proj_scope with proj.
+Open Scope proj_scope.
 
-Notation "a '<=' b" := (projLe a b) (at level 70) : project.
+Notation "a ':+' b" := (Sum a b) (right associativity, at level 55) : proj_scope.
 
-(* Notation "a '>=' b" := (projLe b a) (at level 70) : project. *)
+Notation "a ':>' b" := (Seq a b) (right associativity, at level 45) : proj_scope.
 
-Notation "a '<=>' b" := ((projLe a b) /\ (projLe b a)) (at level 70) : project.
+Notation "a ':*' b" := (Prod a b) (right associativity, at level 35) : proj_scope.
+
+Notation "a '<=' b" := (projLe a b) (at level 70) : proj_scope.
+
+Notation "a '>=' b" := (projGe b a) (at level 70) : proj_scope.
+
+Notation "a '<=>' b" := (projE a b) (at level 70) : proj_scope.
+
+Lemma projESymmetry : forall a b, a <=> b -> b <=> a.
+Proof.
+  unfold projE, projLe, projGe.
+  intros.
+  inversion H.
+  constructor ; assumption.
+Qed.
 
 Lemma leTransitive : forall a b c, a <= b -> b <= c -> a <= c.
 Proof.
@@ -46,7 +62,7 @@ Qed.
 
 Lemma sumSymmetry : forall a b, a :+ b <=> b :+ a.
 Proof.
-  unfold projLe.
+  unfold projE, projLe, projGe.
   split ;
   intros ;
   inversion H ; subst ;
@@ -56,10 +72,10 @@ Qed.
 
 Lemma sumTransitive : forall a b c, a :+ (b :+ c) <= (a :+ b) :+ c .
 Proof.
-  unfold projLe.
+  unfold projE, projLe, projGe.
   intros.
   inversion H ; subst. {
-    inversion H1 ; subst.
+    inversion H4 ; subst.
     - apply ESumLeft. assumption.
     - apply ESumRight. apply ESumLeft. assumption.
   } {
@@ -69,47 +85,50 @@ Qed.
 
 Lemma prodSymmetry : forall a b, a :* b <=> b :* a.
 Proof.
-  unfold projLe.
+  unfold projE, projLe, projGe.
+  intros.
   split;
-    intros ;
-    inversion H ; subst;
+    intros;
+    inversion H;
+    rewrite Nat.min_comm;
+    rewrite Nat.max_comm;
     constructor ; assumption.
 Qed.
 
 Lemma prodTransitive : forall a b c, a :* (b :* c) <=> (a :* b) :* c .
 Proof.
-  unfold projLe.
-  split. {
-    intros.
-    inversion H ; subst.
-    inversion H2 ; subst.
-    constructor ; try assumption ; try (constructor ; assumption).
+  unfold projE, projLe, projGe.
+  intros.
+  split ; intros ; inversion H. {
+    inversion H2. subst a1 b1 loA hiA.
+    rewrite <- Nat.min_assoc.
+    rewrite <- Nat.max_assoc.
+    repeat (constructor ; try assumption).
   } {
-    intros.
-    inversion H ; subst.
-    inversion H3 ; subst.
-    constructor ; try assumption ; try (constructor ; assumption).
+    inversion H5. subst a1 b1 loB hiB.
+    rewrite Nat.min_assoc.
+    rewrite Nat.max_assoc.
+    repeat (constructor ; try assumption).
   }
 Qed.
 
 Lemma sumDistrib : forall a b c, a :* (b :+ c) <=> a :* b :+ a :* c.
 Proof.
-  unfold projLe.
-  split. {
-    intros.
-    inversion H ; subst. {
-      inversion H1 ; subst.
-      - constructor ; try assumption.
-        apply ESumLeft. assumption.
-    } {
-      inversion H1 ; subst.
+  unfold projE, projLe, projGe.
+  intros.
+  split; intros. {
+    inversion H. {
+      inversion H4. subst a1 b1 lo hi.
       constructor ; try assumption.
-      apply ESumRight. assumption.
+      apply ESumLeft ; assumption.
+    } {
+      inversion H4. subst a1 b1 lo hi.
+      constructor ; try assumption.
+      apply ESumRight ; assumption.
     }
   } {
-    intros.
     inversion H ; subst. {
-      inversion H3 ; subst. {
+      inversion H5 ; subst. {
         apply ESumLeft. constructor ; assumption.
       } {
         apply ESumRight. constructor ; assumption.
